src/Renaming.v
@@ -1,61 +1,369 @@
+
 Require Import Label PeanoNat Compare_dec StrictProp.
-Require Import Var Closing.
+Require Import Var.
 
-Definition raw_renaming_pushes : Type :=
-  list (label * list (option var)).
+Inductive raw_renaming :=
+  | raw_renaming_nil : raw_renaming
+  | raw_renaming_cons :
+      option label -> option var
+      -> raw_renaming -> raw_renaming.
 
-Definition is_less_than_renaming_pushes
-           s (r : raw_renaming_pushes) :=
+Fixpoint is_normalized_raw_renaming_entry so vo r :=
   match r with
-  | nil => true
-  | cons (s', ps) r => is_less_than_label s s'
+  | raw_renaming_nil =>
+      negb (var_opt_eqb vo (zero_var_opt so))
+  | raw_renaming_cons so' vo' r =>
+    if label_opt_eqb so so' then true
+    else is_normalized_raw_renaming_entry
+           so (unshift_var_opt vo' vo) r
   end.
 
-Fixpoint is_normalized_raw_renaming_pushes
-         (r : raw_renaming_pushes) :=
+Fixpoint is_normalized_raw_renaming r :=
   match r with
-  | nil => true
-  | cons (s, ps) r =>
-    andb
-      (is_less_than_renaming_pushes s r)
-      (andb
-         (andb (negb (is_pushes_nil ps))
-               (is_normalized_pushes ps))
-         (is_normalized_raw_renaming_pushes r))
+  | raw_renaming_nil => true
+  | raw_renaming_cons so vo r =>
+    andb (is_normalized_raw_renaming_entry so vo r)
+         (is_normalized_raw_renaming r)
   end.
-
-Definition normalized_raw_renaming_pushes r :=
-  if is_normalized_raw_renaming_pushes r then sUnit
-  else sEmpty.
-
-Set Primitive Projections.
-Record raw_renaming :=
-  mk_raw_renaming {
-      r_renaming : raw_renaming_pushes;
-      r_closing : raw_closing;
-    }.
-Add Printing Constructor raw_renaming.
-Unset Primitive Projections.
-
-Definition is_normalized_raw_renaming r :=
-  andb (is_normalized_raw_renaming_pushes (r_renaming r))
-       (is_normalized_pushes (r_closing r)).
 
 Definition normalized_raw_renaming r :=
   if is_normalized_raw_renaming r then sUnit
   else sEmpty.
 
+Definition normalized_raw_renaming_from_cons {so vo r} :
+  normalized_raw_renaming (raw_renaming_cons so vo r) ->
+  normalized_raw_renaming r.
+Proof.
+  unfold normalized_raw_renaming; cbn.
+  destruct (is_normalized_raw_renaming r); try easy.
+  rewrite Bool.andb_false_r; easy.
+Qed.
+
 Set Primitive Projections.
 Record renaming :=
   mk_renaming {
       r_raw : raw_renaming;
-      r_normalized : normalized_raw_renaming r_raw;
+      r_normalized : normalized_raw_renaming r_raw
     }.
 Add Printing Constructor renaming.
 Unset Primitive Projections.
 
+Definition renaming_id : renaming :=
+  mk_renaming raw_renaming_nil stt.
+
+Fixpoint raw_renaming_cons_null_entry so vo r :=
+  match r with
+  | raw_renaming_nil =>
+      if (var_opt_eqb vo zero_var_opt) then Some r
+      else None
+  | raw_renaming_cons so' vo' r =>
+    if label_opt_eqb so so' then None
+    else
+      match raw_renaming_cons_null_entry
+              so (unshift_var_opt vo' vo) r with
+      | None => None
+      | Some r =>
+        Some (raw_renaming_cons so' (shift_var_opt vo vo') r)
+      end
+  end.
+
+Definition normalized_raw_renaming_cons so vo r :=
+  match raw_renaming_cons_null_entry so vo r with
+  | Some r => r
+  | None => raw_renaming_cons so vo r
+  end.
+
+Definition var_opt_geb vo1 vo2 :=
+  match vo1, vo2 with
+  | free n1, free n2 -> name_geb n1 n2
+  | bound l1, bound l1 -> level_geb l1 l2
+  | free _, bound _ -> false
+  | bound _, free _ -> false
+  end.
 
 
+Definition var_nonzero vo :=
+    negb (var_opt_eqb vo zero_var_opt) = true.
+
+Definition var_nonzero_shift vo1 vo2 :
+  var_nonzero vo2 ->
+  var_nonzero (shift_var_opt vo1 vo2).
+Proof.
+  destruct vo1 as [[n1|[|l1]]|], vo2 as [[n2|[|l2]]|];
+    cbn; try easy.
+  unfold shift_level.
+  destruct (le_gt_dec (S l1) (S l2)); easy.
+Defined.
+
+Definition var_nonzero_unshift vo1 vo2 vo3 :
+  (var_nonzero vo1 -> var_nonzero vo2) ->
+  var_nonzero (unshift_var_opt vo3 vo1) ->
+  var_nonzero (unshift_var_opt vo3 vo2).
+Proof.
+  destruct vo1 as [[n1|[|l1]]|], vo2 as [[n2|[|l2]]|],
+    vo3 as [[n3|[|l3]]|]; cbn; try easy.
+
+Definition is_normalized_raw_renaming_entry_greater so vo1 vo2 r :
+  (var_nonzero vo1 -> var_nonzero vo2) ->
+  is_normalized_raw_renaming_entry so vo1 r = true ->
+  is_normalized_raw_renaming_entry so vo2 r = true.
+Proof.
+  generalize dependent vo1.
+  generalize dependent vo2.
+  induction r as [|so2 vo3]; intros vo2 vo1; cbn; try easy.
+  destruct (label_opt_eqb so so2); try easy.
+  intros Himp.
+  apply IHr.
 
 
+Definition var_nonzero_unshift vo1 vo2 :
+  var_nonzero (unshift_var_opt vo1 vo2) ->
+  var_nonzero vo1 \/ var_nonzero vo2
+Proof.
+  split; intros H.
+  - destruct vo1 as [[n1|[|l1]]|], vo2 as [[n2|[|l2]]|];
+      cbn; try easy; destruct H; try easy.
 
+  split.
+
+Definition is_normalized_raw_renaming_entry_unshift_shift
+           so vo1 vo2 vo3 r :
+  is_normalized_raw_renaming_entry so
+    (unshift_var_opt vo3 vo1) r = true ->
+  is_normalized_raw_renaming_entry so
+    (unshift_var_opt (shift_var_opt vo2 vo3) vo1) r = true.
+Proof.
+  induction r as [|so2 vo4]; cbn.
+  - admit.
+  - destruct (label_opt_eqb so so2); try easy.
+    
+
+Definition raw_renaming_cons_null_entry_preserves_entries
+           so1 vo1 r1 r2 so2 vo2 :
+  is_normalized_raw_renaming_entry so1 vo1 r1 = true ->
+  raw_renaming_cons_null_entry so2 vo2 r1 = Some r2 ->
+  is_normalized_raw_renaming_entry so1 vo1 r2 = true.
+Proof.
+  generalize dependent vo1.
+  generalize dependent vo2.
+  generalize dependent r2.
+  induction r1 as [|so3 vo3]; intros r2 vo2 vo1; cbn.
+  - destruct (var_opt_eqb vo2 zero_var_opt); try easy; intros.
+    assert (r2 = raw_renaming_nil) as Hrw by congruence.
+    rewrite Hrw; easy.
+  - destruct (label_opt_eqb so2 so3) eqn:Heq1; try easy.
+    destruct (raw_renaming_cons_null_entry so2
+                (unshift_var_opt vo3 vo2) r1) eqn:Heq2; try easy.
+    intros;
+      assert (r2 = raw_renaming_cons so3 (shift_var_opt vo2 vo3) r)
+      as Hrw by congruence; rewrite Hrw; cbn.
+    destruct (label_opt_eqb so1 so3); try easy.
+    apply IHr1 with (vo2 := unshift_var_opt vo3 vo2); try easy.
+
+Definition raw_renaming_cons_null_entry_some so vo r r' :
+  normalized_raw_renaming r ->
+  raw_renaming_cons_null_entry so vo r = Some r' ->
+  normalized_raw_renaming r'.
+  generalize dependent so.
+  generalize dependent vo.
+  generalize dependent r'.
+  induction r as [|so' vo' r]; intros r' vo so; cbn.
+  - destruct (var_opt_eqb vo zero_var_opt); try easy.
+    intros; assert (r' = raw_renaming_nil)
+      as Hrw by congruence.
+    rewrite Hrw; easy.
+  - destruct (label_opt_eqb so so'); try easy.
+    destruct (raw_renaming_cons_null_entry so
+                (unshift_var_opt vo' vo) r) eqn:Heq;
+      try easy.
+    apply IHr in Heq.
+    
+Defined.
+
+Definition raw_renaming_cons_null_entry_none so vo r r' :
+  raw_renaming_cons_null_entry so vo r = None ->
+  is_normalized_raw_renaming_entry so vo r.
+Defined.
+
+Definition normalized_raw_renaming_cons_normalized
+           {so vo r} :
+  normalized_raw_renaming r ->
+  normalized_raw_renaming
+    (normalized_raw_renaming_cons so vo r).
+Proof. destruct vo as [[|[]]|], r; easy. Defined.
+
+Definition closing_cons0 vo r :=
+  mkclosing
+    (normalized_pushes_cons vo (c_raw r))
+    (normalized_pushes_cons_normalized
+       (c_normalized r)).
+
+Definition closing_weak0 r :=
+  closing_cons0 None r.
+
+Definition closing_exchange0 r l :=
+  closing_cons0 (Some (bound l)) r.
+
+Definition closing_close0 r n :=
+  closing_cons0 (Some (free n)) r.
+
+Definition raw_closing_hd r :=
+  match r with
+  | nil => zero_var_opt
+  | cons vo' _ => vo'
+  end.
+
+Definition raw_closing_tl (r : raw_closing) :=
+  match r with
+  | nil => nil
+  | cons _ r' => r'
+  end.
+
+Fixpoint raw_closing_cons l vo r :=
+  match l with
+  | 0 => normalized_pushes_cons vo r
+  | S l =>
+    normalized_pushes_cons
+      (shift_var_opt vo (raw_closing_hd r))
+      (raw_closing_cons
+         l (unshift_var_opt (raw_closing_hd r) vo)
+         (raw_closing_tl r))
+  end.
+
+Definition raw_closing_cons_normalized {l vo r} :
+  normalized_pushes r ->
+  normalized_pushes (raw_closing_cons l vo r).
+Proof.
+  generalize dependent vo.
+  generalize dependent r.
+  induction l; cbn; intros r vo Hnorm;
+    apply normalized_pushes_cons_normalized; try easy.
+  apply IHl.
+  destruct r as [|vo' r]; try easy.
+  apply normalized_pushes_from_cons in Hnorm; easy.
+Defined.
+
+Definition closing_cons l vo r :=
+  mkclosing
+    (raw_closing_cons l vo (c_raw r))
+    (raw_closing_cons_normalized (c_normalized r)).
+
+Definition closing_weak l r :=
+  closing_cons l None r.
+
+Definition closing_exchange l1 l2 r :=
+  closing_cons l1 (Some (bound l2)) r.
+
+Definition closing_close l n r :=
+  closing_cons l (Some (free n)) r.
+
+Fixpoint closing_weak_n N : closing :=
+  match N with
+  | 0 => closing_id
+  | S N => closing_weak 0 (closing_weak_n N)
+  end.
+
+Fixpoint closing_weakening N M : closing :=
+  match N with
+  | 0 => closing_weak_n M
+  | S N => closing_exchange 0 0 (closing_weakening N M)
+  end.
+
+Fixpoint apply_raw_closing_var r : var_op :=
+  match r with
+  | nil => var_op_id
+  | cons vo r =>
+    lift_var_op (apply_raw_closing_var r) @ push_var vo
+  end.
+
+Definition apply_closing_var r :=
+  apply_raw_closing_var (c_raw r).
+
+Set Primitive Projections.
+Record closing_rhs :=
+  mk_closing_rhs {
+      rhs_raw_closing : raw_closing;
+      rhs_push : option var
+    }.
+Add Printing Constructor closing_rhs.
+Unset Primitive Projections.
+
+Definition normalized_closing_rhs r :=
+  normalized_pushes (rhs_raw_closing r).
+
+Definition closing_rhs_cons0 vo r :=
+  mk_closing_rhs
+    (normalized_pushes_cons
+       (unshift_var_opt (rhs_push r) vo)
+       (rhs_raw_closing r))
+    (shift_var_opt vo (rhs_push r)).
+
+Definition closing_rhs_weak0 r :=
+  closing_rhs_cons0 None r.
+
+Definition closing_rhs_exchange0 l r :=
+  closing_rhs_cons0 (Some (bound l)) r.
+
+Definition closing_rhs_close0 n r :=
+  closing_rhs_cons0 (Some (free n)) r.
+
+Definition closing_rhs_cons0_normalized {vo r} :
+  normalized_closing_rhs r ->
+  normalized_closing_rhs (closing_rhs_cons0 vo r).
+Proof.
+  destruct r as [? []]; cbn;
+    apply normalized_pushes_cons_normalized;
+    easy.
+Defined.
+
+Fixpoint transpose_push_raw_closing vo r {struct r} :=
+  match r with
+  | nil => mk_closing_rhs nil vo
+  | cons vo' r =>
+    if var_opt_eqb vo zero_var_opt then mk_closing_rhs r vo'
+    else closing_rhs_cons0 vo'
+           (transpose_push_raw_closing
+              (unshift_var_var_opt zero_var vo) r)
+  end.
+
+Definition transpose_push_raw_closing_normalized {vo r} :
+  normalized_pushes r ->
+  normalized_closing_rhs
+    (transpose_push_raw_closing vo r).
+Proof.
+  generalize dependent vo.
+  induction r as [|vo' r]; intros vo norm; try easy; cbn.
+  apply normalized_pushes_from_cons in norm.
+  destruct (var_opt_eqb vo zero_var_opt); try easy.
+  apply closing_rhs_cons0_normalized.
+  apply IHr; easy.
+Defined.
+
+Fixpoint compose_raw_closing r1 r2 :=
+  match r1 with
+  | nil => r2
+  | cons vo r1 =>
+    let rhs := transpose_push_raw_closing vo r2 in
+    normalized_pushes_cons
+      (rhs_push rhs)
+      (compose_raw_closing r1 (rhs_raw_closing rhs))
+  end.
+
+Definition compose_raw_closing_normalized {r1 r2} :
+  normalized_pushes r1 ->
+  normalized_pushes r2 ->
+  normalized_pushes (compose_raw_closing r1 r2).
+Proof.
+  generalize dependent r2.
+  induction r1 as [|vo]; intros r2 norm1 norm2; try easy.
+  apply normalized_pushes_from_cons in norm1; cbn.
+  apply normalized_pushes_cons_normalized.
+  apply IHr1; try easy.
+  apply transpose_push_raw_closing_normalized; easy.
+Defined.
+
+Definition compose_closing r1 r2 :=
+  mkclosing
+    (compose_raw_closing (c_raw r1) (c_raw r2))
+    (compose_raw_closing_normalized
+       (c_normalized r1) (c_normalized r2)).
